more

src/Rupicola/Examples/ConstantTime/CMoveLeakage.v
@@ -1,12 +1,14 @@
 Require Import Rupicola.Examples.CMove.CMove.
 Require Import Rupicola.Examples.Cells.Cells.
-From Stdlib Require Import ZArith.ZArith Strings.String.
+From Stdlib Require Import ZArith.ZArith Strings.String Lia.
 Require Import coqutil.Word.Bitwidth coqutil.Word.Interface.
+Require Import coqutil.Word.Properties.
 Require Import coqutil.Map.Interface coqutil.Byte.
 Require Import coqutil.Map.Properties.
 Require Import bedrock2.LeakageSemantics.
 Require Import bedrock2.LeakageWeakestPrecondition.
 Require Import bedrock2.LeakageProgramLogic.
+Require Import bedrock2.LeakageLoops.
 Require Import bedrock2.Map.SeparationLogic.
 
 Import List.ListNotations.
@@ -14,6 +16,21 @@ Import LeakageProgramLogic.Coercions.
 Import SeparationLogic.
 Local Open Scope string_scope.
 Local Open Scope list_scope.
+
+(* Keep symbolic execution from eagerly decomposing a loop invariant.  The
+   sealed implementation is logically the identity, but tactics cannot unfold
+   it while executing the generated loop body. *)
+Module Type LeakageProofFenceSig.
+  Parameter t : Prop -> Prop.
+  Parameter intro : forall P, P -> t P.
+  Parameter elim : forall P, t P -> P.
+End LeakageProofFenceSig.
+
+Module LeakageProofFence : LeakageProofFenceSig.
+  Definition t (P : Prop) : Prop := P.
+  Definition intro P : P -> t P := fun H => H.
+  Definition elim P : t P -> P := fun H => H.
+End LeakageProofFence.
 
 Section WithParameters.
   Context {width: Z} {BW: Bitwidth width}.
@@ -54,6 +71,16 @@ Section WithParameters.
             (rewrite ?map.get_put_dec, ?map.get_empty,
                      ?word.of_Z_unsigned; cbn)).
 
+  Local Ltac normalize_generated_map_get :=
+    repeat first
+      [ rewrite map.get_put_dec
+      | rewrite map.get_remove_dec
+      | rewrite map.get_empty
+      | match goal with
+        | |- context [@map.get _ _ _ ?m _] =>
+            is_var m; cbv delta [m]
+        end ].
+
   Definition cmove_word_leakage_spec : spec_of "cmove_word" :=
     fnspec! "cmove_word" (mask ptr1 ptr2 : word) /
       (c1 c2 : cell) (R : mem -> Prop),
@@ -90,5 +117,496 @@ Section WithParameters.
         cswap_word_leakage_spec functions).
   Proof.
     prove_word_leakage.
+  Qed.
+
+  Definition word_array_stride : word :=
+    word.of_Z (Z.of_nat (@Memory.bytes_per width Syntax.access_size.word)).
+
+  Definition word_array_index (base : word) (i : nat) : word :=
+    word.add base
+      (word.of_Z (word.unsigned word_array_stride * Z.of_nat i)).
+
+  Definition initialized_word (addr : word) (_ : unit) : mem -> Prop :=
+    Lift1Prop.ex1 (fun value => Scalars.scalar addr value).
+
+  Definition initialized_word_array (base : word) (n : nat) : mem -> Prop :=
+    Array.array initialized_word word_array_stride base (List.repeat tt n).
+
+  Definition array_loop_locals
+      (mask len ptr1 ptr2 from nmask index : word) : locals :=
+    map.put
+      (map.put
+        (map.put
+          (map.put
+            (map.put
+              (map.put
+                (map.put
+                  (map.put map.empty "mask" mask) "len" len)
+                "a1" ptr1)
+              "a2" ptr2)
+            "from" from)
+          "nmask" nmask)
+        "_gs_from0" index)
+      "_gs_to0" len.
+
+  Lemma word_of_Z_nat_succ i :
+    (word.add (word.of_Z (Z.of_nat i)) (word.of_Z 1) : word) =
+    word.of_Z (Z.of_nat (S i)).
+  Proof.
+    rewrite <- word.ring_morph_add.
+    f_equal; lia.
+  Qed.
+
+  Lemma word_array_index_as_mul base i :
+    word_array_index base i =
+    word.add base (word.mul word_array_stride (word.of_Z (Z.of_nat i))).
+  Proof.
+    unfold word_array_index.
+    rewrite word.ring_morph_mul, word.of_Z_unsigned.
+    reflexivity.
+  Qed.
+
+  Lemma initialized_word_array_index base n i (H : (i < n)%nat) :
+    Lift1Prop.iff1
+      (initialized_word_array base n)
+      (Array.array initialized_word word_array_stride base
+         (List.firstn i (List.repeat tt n))
+       * (initialized_word (word_array_index base i)
+            (List.hd tt (List.skipn i (List.repeat tt n)))
+          * Array.array initialized_word word_array_stride
+              (word.add (word_array_index base i) word_array_stride)
+              (List.skipn (S i) (List.repeat tt n))))%sep.
+  Proof.
+    unfold initialized_word_array, word_array_index.
+    eapply Array.array_index_nat_inbounds.
+    rewrite List.repeat_length; exact H.
+  Qed.
+
+  Definition cmove_array_one_iteration_leakage
+      (ptr1 ptr2 : word) (i : nat) : leakage :=
+    [leak_word (word_array_index ptr1 i);
+     leak_word (word_array_index ptr2 i);
+     leak_word (word_array_index ptr1 i);
+     leak_bool true].
+
+  Fixpoint cmove_array_iterations_leakage
+      (ptr1 ptr2 : word) (count : nat) : leakage :=
+    match count with
+    | O => []
+    | S count' =>
+        cmove_array_one_iteration_leakage ptr1 ptr2 count' ++
+        cmove_array_iterations_leakage ptr1 ptr2 count'
+    end.
+
+  Definition cmove_array_public_leakage
+      (ptr1 ptr2 : word) (n : nat) : leakage :=
+    leak_bool false :: cmove_array_iterations_leakage ptr1 ptr2 n.
+
+  Definition cswap_array_one_iteration_leakage
+      (ptr1 ptr2 : word) (i : nat) : leakage :=
+    [leak_word (word_array_index ptr2 i);
+     leak_word (word_array_index ptr1 i);
+     leak_word (word_array_index ptr2 i);
+     leak_word (word_array_index ptr1 i);
+     leak_bool true].
+
+  Fixpoint cswap_array_iterations_leakage
+      (ptr1 ptr2 : word) (count : nat) : leakage :=
+    match count with
+    | O => []
+    | S count' =>
+        cswap_array_one_iteration_leakage ptr1 ptr2 count' ++
+        cswap_array_iterations_leakage ptr1 ptr2 count'
+    end.
+
+  Definition cswap_array_public_leakage
+      (ptr1 ptr2 : word) (n : nat) : leakage :=
+    leak_bool false :: cswap_array_iterations_leakage ptr1 ptr2 n.
+
+  Definition cmove_array_leakage_spec : spec_of "cmove_array" :=
+    fnspec! "cmove_array" (mask len ptr1 ptr2 : word) /
+      (n : nat) (R : mem -> Prop),
+      { requires k t m :=
+          word.unsigned len = Z.of_nat n /\
+          (initialized_word_array ptr1 n
+           * initialized_word_array ptr2 n * R)%sep m;
+        ensures k' t' m' :=
+          k' = cmove_array_public_leakage ptr1 ptr2 n ++ k /\
+          t' = t }.
+
+  Definition cswap_array_leakage_spec : spec_of "cswap_array" :=
+    fnspec! "cswap_array" (mask len ptr1 ptr2 : word) /
+      (n : nat) (R : mem -> Prop),
+      { requires k t m :=
+          word.unsigned len = Z.of_nat n /\
+          (initialized_word_array ptr1 n
+           * initialized_word_array ptr2 n * R)%sep m;
+        ensures k' t' m' :=
+          k' = cswap_array_public_leakage ptr1 ptr2 n ++ k /\
+          t' = t }.
+
+  Lemma cmove_array_leakage_ok :
+    program_logic_goal_for (@cmove_array_br2fn width word)
+      (forall functions : Semantics.env,
+        map.get functions "cmove_array" =
+          Some (@cmove_array_br2fn width word) ->
+        cmove_array_leakage_spec functions).
+  Proof.
+    prove_word_leakage.
+    lazymatch goal with
+    | |- LeakageSemantics.exec ?functions
+           (Syntax.cmd.while ?condition ?body) ?K ?T ?M ?L ?post =>
+        change (LeakageWeakestPrecondition.cmd functions
+                  (Syntax.cmd.while condition body) K T M L post)
+    end.
+    eapply LeakageLoops.wp_while.
+    eexists nat, Nat.lt,
+      (fun remaining K T M L =>
+         exists i nmask,
+           (i <= n)%nat /\
+           map.get L "mask" = Some mask /\
+           map.get L "len" = Some len /\
+           map.get L "a1" = Some ptr1 /\
+           map.get L "a2" = Some ptr2 /\
+           map.get L "nmask" = Some nmask /\
+           map.get L "_gs_from0" = Some (word.of_Z (Z.of_nat i)) /\
+           map.get L "_gs_to0" = Some len /\
+           L = array_loop_locals mask len ptr1 ptr2 from nmask
+                 (word.of_Z (Z.of_nat i)) /\
+           K = cmove_array_iterations_leakage ptr1 ptr2 i ++ k /\
+           T = t /\
+           (initialized_word_array ptr1 n
+            * initialized_word_array ptr2 n * R)%sep M /\
+           remaining = (n - i)%nat).
+    split.
+    { eapply Wf_nat.lt_wf. }
+    split.
+    { exists n, O. eexists.
+      assert (_gs_from0 = word.of_Z 0) as Hgs0.
+      { subst _gs_from0; apply word.of_Z_unsigned. }
+      subst _gs_from0; subst l3; subst l2; subst l1; subst l0; subst l.
+      repeat split; try assumption; try reflexivity.
+      all: repeat (rewrite ?map.get_put_dec, ?map.get_empty; cbn).
+      all: try unfold array_loop_locals.
+      all: repeat rewrite Hgs0.
+      all: try rewrite word.of_Z_unsigned.
+      all: cbn [cmove_array_iterations_leakage List.app].
+      all: try reflexivity.
+      all: try apply Nat.le_0_l.
+      all: try ecancel_assumption.
+      all: try lia.
+      all: reflexivity. }
+    intros remaining K T M L
+      (i & nmask & Hi & Hmask & Hlen & Ha1 & Ha2 & Hnmask &
+       Hindex & Hbound & Hlocals & HK & HT & HM & Hremaining).
+    eexists (if word.ltu (word.of_Z (Z.of_nat i)) len
+             then word.of_Z 1 else word.of_Z 0), K.
+    split.
+    { eexists; split; [exact Hindex|].
+      eexists; split; [exact Hbound|].
+      cbn [LeakageSemantics.leak_binop Semantics.interp_binop].
+      split; reflexivity. }
+    split.
+    { intro Hnonzero.
+      destruct (word.ltu (word.of_Z (Z.of_nat i)) len) eqn:Hltu.
+      2: rewrite word.unsigned_of_Z_0 in Hnonzero; contradiction.
+      assert (Hindex_range :
+                0 <= Z.of_nat i < 2 ^ width).
+      { pose proof (word.unsigned_range len). lia. }
+      assert (Hlt : (i < n)%nat).
+      { rewrite Interface.word.unsigned_ltu in Hltu.
+        rewrite word.unsigned_of_Z_nowrap in Hltu by exact Hindex_range.
+        apply Z.ltb_lt in Hltu. lia. }
+      unfold array_loop_locals in Hlocals.
+      subst L.
+      SeparationLogic.seprewrite_in
+        (initialized_word_array_index ptr1 n i Hlt) HM.
+      SeparationLogic.seprewrite_in
+        (initialized_word_array_index ptr2 n i Hlt) HM.
+      unfold initialized_word, word_array_index in HM.
+      repeat rewrite word.ring_morph_mul, word.of_Z_unsigned in HM.
+      extract_ex1_and_emp_in_hyps.
+      lazymatch goal with
+      | body := context[
+          Syntax.cmd.set "v1"
+            (Syntax.expr.load Syntax.access_size.word
+              (Syntax.expr.op Syntax.bopname.add _
+                (Syntax.expr.op Syntax.bopname.mul
+                  (Syntax.expr.literal ?stride) _)))] |- _ =>
+          assert (word.of_Z stride = word_array_stride) as Hstride
+            by reflexivity;
+          rewrite <- Hstride in HM
+      end.
+      lazymatch goal with
+      | |- LeakageWeakestPrecondition.cmd ?fs ?body ?K0 ?T0 ?M0 ?L0 ?post =>
+          eapply LeakageWeakestPreconditionProperties.weaken_cmd
+            with (post1 := fun K1 T1 M1 L1 =>
+              LeakageProofFence.t (post K1 T1 M1 L1))
+      end.
+      2: { intros K1 T1 M1 L1 Hpost.
+           exact (LeakageProofFence.elim _ Hpost). }
+      prove_word_leakage.
+      all: try lazymatch goal with
+      | |- @map.get _ _ _ _ _ = _ =>
+          normalize_generated_map_get;
+          cbn;
+          reflexivity
+      end.
+      apply LeakageProofFence.intro.
+      exists (n - S i)%nat.
+      split; [|lia].
+      exists (S i), nmask.
+      repeat split.
+      all: try lia.
+      all: try reflexivity.
+      all: try lazymatch goal with
+      | |- @map.get _ _ _ _ _ = _ =>
+          normalize_generated_map_get;
+          rewrite ?word_of_Z_nat_succ;
+          cbn;
+          reflexivity
+      end.
+      - unfold array_loop_locals.
+        apply map.map_ext; intros key.
+        normalize_generated_map_get.
+        repeat rewrite word_of_Z_nat_succ.
+        repeat first
+          [ rewrite map.get_put_dec
+          | rewrite map.get_remove_dec
+          | rewrite map.get_empty
+          | match goal with
+            | |- context [if ?test then _ else _] =>
+                destr.destr test; try congruence
+            end ].
+      - lazymatch type of Hstride with
+        | ?generated_stride = word_array_stride =>
+            change
+              (leak_word
+                 (word.add ptr1
+                    (word.mul generated_stride (word.of_Z (Z.of_nat i)))) ::
+               leak_word
+                 (word.add ptr2
+                    (word.mul generated_stride (word.of_Z (Z.of_nat i)))) ::
+               leak_word
+                 (word.add ptr1
+                    (word.mul generated_stride (word.of_Z (Z.of_nat i)))) ::
+               leak_bool true ::
+                 cmove_array_iterations_leakage ptr1 ptr2 i ++ k =
+               cmove_array_iterations_leakage ptr1 ptr2 (S i) ++ k)
+        end.
+        cbn [cmove_array_iterations_leakage
+             cmove_array_one_iteration_leakage List.app].
+        repeat rewrite word_array_index_as_mul.
+        rewrite <- Hstride.
+        reflexivity.
+      - SeparationLogic.seprewrite
+          (initialized_word_array_index ptr1 n i Hlt).
+        SeparationLogic.seprewrite
+          (initialized_word_array_index ptr2 n i Hlt).
+        unfold initialized_word.
+        repeat rewrite word_array_index_as_mul.
+        rewrite <- Hstride.
+        extract_ex1_and_emp_in_goal.
+        ecancel_assumption.
+    }
+    intro Hzero.
+    destruct (word.ltu (word.of_Z (Z.of_nat i)) len) eqn:Hltu.
+    { rewrite word.unsigned_of_Z_1 in Hzero; lia. }
+    assert (Hindex_range : 0 <= Z.of_nat i < 2 ^ width).
+    { pose proof (word.unsigned_range len). lia. }
+    assert (Hi_eq : (i = n)%nat).
+    { rewrite Interface.word.unsigned_ltu in Hltu.
+      rewrite word.unsigned_of_Z_nowrap in Hltu by exact Hindex_range.
+      apply Z.ltb_ge in Hltu.
+      lia. }
+    subst i.
+    split; [reflexivity|].
+    split.
+    - rewrite HK; reflexivity.
+    - exact HT.
+  Qed.
+
+  Lemma cswap_array_leakage_ok :
+    program_logic_goal_for (@cswap_array_br2fn width word)
+      (forall functions : Semantics.env,
+        map.get functions "cswap_array" =
+          Some (@cswap_array_br2fn width word) ->
+        cswap_array_leakage_spec functions).
+  Proof.
+    prove_word_leakage.
+    lazymatch goal with
+    | |- LeakageSemantics.exec ?functions
+           (Syntax.cmd.while ?condition ?body) ?K ?T ?M ?L ?post =>
+        change (LeakageWeakestPrecondition.cmd functions
+                  (Syntax.cmd.while condition body) K T M L post)
+    end.
+    eapply LeakageLoops.wp_while.
+    eexists nat, Nat.lt,
+      (fun remaining K T M L =>
+         exists i nmask,
+           (i <= n)%nat /\
+           map.get L "mask" = Some mask /\
+           map.get L "len" = Some len /\
+           map.get L "a1" = Some ptr1 /\
+           map.get L "a2" = Some ptr2 /\
+           map.get L "nmask" = Some nmask /\
+           map.get L "_gs_from0" = Some (word.of_Z (Z.of_nat i)) /\
+           map.get L "_gs_to0" = Some len /\
+           L = array_loop_locals mask len ptr1 ptr2 from nmask
+                 (word.of_Z (Z.of_nat i)) /\
+           K = cswap_array_iterations_leakage ptr1 ptr2 i ++ k /\
+           T = t /\
+           (initialized_word_array ptr1 n
+            * initialized_word_array ptr2 n * R)%sep M /\
+           remaining = (n - i)%nat).
+    split.
+    { eapply Wf_nat.lt_wf. }
+    split.
+    { exists n, O. eexists.
+      assert (_gs_from0 = word.of_Z 0) as Hgs0.
+      { subst _gs_from0; apply word.of_Z_unsigned. }
+      subst _gs_from0; subst l3; subst l2; subst l1; subst l0; subst l.
+      repeat split; try assumption; try reflexivity.
+      all: repeat (rewrite ?map.get_put_dec, ?map.get_empty; cbn).
+      all: try unfold array_loop_locals.
+      all: repeat rewrite Hgs0.
+      all: try rewrite word.of_Z_unsigned.
+      all: cbn [cswap_array_iterations_leakage List.app].
+      all: try reflexivity.
+      all: try apply Nat.le_0_l.
+      all: try ecancel_assumption.
+      all: try lia.
+      all: reflexivity. }
+    intros remaining K T M L
+      (i & nmask & Hi & Hmask & Hlen & Ha1 & Ha2 & Hnmask &
+       Hindex & Hbound & Hlocals & HK & HT & HM & Hremaining).
+    eexists (if word.ltu (word.of_Z (Z.of_nat i)) len
+             then word.of_Z 1 else word.of_Z 0), K.
+    split.
+    { eexists; split; [exact Hindex|].
+      eexists; split; [exact Hbound|].
+      cbn [LeakageSemantics.leak_binop Semantics.interp_binop].
+      split; reflexivity. }
+    split.
+    { intro Hnonzero.
+      destruct (word.ltu (word.of_Z (Z.of_nat i)) len) eqn:Hltu.
+      2: rewrite word.unsigned_of_Z_0 in Hnonzero; contradiction.
+      assert (Hindex_range :
+                0 <= Z.of_nat i < 2 ^ width).
+      { pose proof (word.unsigned_range len). lia. }
+      assert (Hlt : (i < n)%nat).
+      { rewrite Interface.word.unsigned_ltu in Hltu.
+        rewrite word.unsigned_of_Z_nowrap in Hltu by exact Hindex_range.
+        apply Z.ltb_lt in Hltu. lia. }
+      unfold array_loop_locals in Hlocals.
+      subst L.
+      SeparationLogic.seprewrite_in
+        (initialized_word_array_index ptr1 n i Hlt) HM.
+      SeparationLogic.seprewrite_in
+        (initialized_word_array_index ptr2 n i Hlt) HM.
+      unfold initialized_word, word_array_index in HM.
+      repeat rewrite word.ring_morph_mul, word.of_Z_unsigned in HM.
+      extract_ex1_and_emp_in_hyps.
+      lazymatch goal with
+      | body := context[
+          Syntax.cmd.set "v1"
+            (Syntax.expr.load Syntax.access_size.word
+              (Syntax.expr.op Syntax.bopname.add _
+                (Syntax.expr.op Syntax.bopname.mul
+                  (Syntax.expr.literal ?stride) _)))] |- _ =>
+          assert (word.of_Z stride = word_array_stride) as Hstride
+            by reflexivity;
+          rewrite <- Hstride in HM
+      end.
+      lazymatch goal with
+      | |- LeakageWeakestPrecondition.cmd ?fs ?body ?K0 ?T0 ?M0 ?L0 ?post =>
+          eapply LeakageWeakestPreconditionProperties.weaken_cmd
+            with (post1 := fun K1 T1 M1 L1 =>
+              LeakageProofFence.t (post K1 T1 M1 L1))
+      end.
+      2: { intros K1 T1 M1 L1 Hpost.
+           exact (LeakageProofFence.elim _ Hpost). }
+      prove_word_leakage.
+      all: try lazymatch goal with
+      | |- @map.get _ _ _ _ _ = _ =>
+          normalize_generated_map_get;
+          cbn;
+          reflexivity
+      end.
+      apply LeakageProofFence.intro.
+      exists (n - S i)%nat.
+      split; [|lia].
+      exists (S i), nmask.
+      repeat split.
+      all: try lia.
+      all: try reflexivity.
+      all: try lazymatch goal with
+      | |- @map.get _ _ _ _ _ = _ =>
+          normalize_generated_map_get;
+          rewrite ?word_of_Z_nat_succ;
+          cbn;
+          reflexivity
+      end.
+      - unfold array_loop_locals.
+        apply map.map_ext; intros key.
+        normalize_generated_map_get.
+        repeat rewrite word_of_Z_nat_succ.
+        repeat first
+          [ rewrite map.get_put_dec
+          | rewrite map.get_remove_dec
+          | rewrite map.get_empty
+          | match goal with
+            | |- context [if ?test then _ else _] =>
+                destr.destr test; try congruence
+            end ].
+      - lazymatch type of Hstride with
+        | ?generated_stride = word_array_stride =>
+            change
+              (leak_word
+                 (word.add ptr2
+                    (word.mul generated_stride (word.of_Z (Z.of_nat i)))) ::
+               leak_word
+                 (word.add ptr1
+                    (word.mul generated_stride (word.of_Z (Z.of_nat i)))) ::
+               leak_word
+                 (word.add ptr2
+                    (word.mul generated_stride (word.of_Z (Z.of_nat i)))) ::
+               leak_word
+                 (word.add ptr1
+                    (word.mul generated_stride (word.of_Z (Z.of_nat i)))) ::
+               leak_bool true ::
+                 cswap_array_iterations_leakage ptr1 ptr2 i ++ k =
+               cswap_array_iterations_leakage ptr1 ptr2 (S i) ++ k)
+        end.
+        cbn [cswap_array_iterations_leakage
+             cswap_array_one_iteration_leakage List.app].
+        repeat rewrite word_array_index_as_mul.
+        rewrite <- Hstride.
+        reflexivity.
+      - SeparationLogic.seprewrite
+          (initialized_word_array_index ptr1 n i Hlt).
+        SeparationLogic.seprewrite
+          (initialized_word_array_index ptr2 n i Hlt).
+        unfold initialized_word.
+        repeat rewrite word_array_index_as_mul.
+        rewrite <- Hstride.
+        extract_ex1_and_emp_in_goal.
+        ecancel_assumption.
+    }
+    intro Hzero.
+    destruct (word.ltu (word.of_Z (Z.of_nat i)) len) eqn:Hltu.
+    { rewrite word.unsigned_of_Z_1 in Hzero; lia. }
+    assert (Hindex_range : 0 <= Z.of_nat i < 2 ^ width).
+    { pose proof (word.unsigned_range len). lia. }
+    assert (Hi_eq : (i = n)%nat).
+    { rewrite Interface.word.unsigned_ltu in Hltu.
+      rewrite word.unsigned_of_Z_nowrap in Hltu by exact Hindex_range.
+      apply Z.ltb_ge in Hltu.
+      lia. }
+    subst i.
+    split; [reflexivity|].
+    split.
+    - rewrite HK; reflexivity.
+    - exact HT.
   Qed.
 End WithParameters.
